# Sum of Alternating Series 1 of from [-1+2-3+4...]

This document explains how to find the sum of the first \( n \) terms of the series:

$$
-1 + 2 - 3 + 4 - 5 + \ldots
$$

## Formula

To find the sum of the first \( n \) terms of this series, you can use the following formula:

$$
S_n = \left\{
\begin{array}{ll}
\frac{n}{2} & \text{if } n \text{ is even} \\
-\frac{n+1}{2} & \text{if } n \text{ is odd}
\end{array}
\right.
$$



### Examples

1. For \( n = 6 \) (even):
   $$
   S_6 = \frac{6}{2} = 3
   $$

2. For \( n = 5 \) (odd):
   $$
   S_5 = -\frac{5+1}{2} = -3
   $$

***
***
***
***
# Sum of Alternating Series of from [1-2+3-4...]


This document explains how to find the sum of the first \( n \) terms of the series:

$$
1 - 2 + 3 - 4 + 5 - 6 + \ldots
$$

## Formula

To find the sum of the first \( n \) terms of this series, you can use the following formula:

$$
S_n = \left\{
\begin{array}{ll}
-\frac{n}{2} & \text{if } n \text{ is even} \\
\frac{n+1}{2} & \text{if } n \text{ is odd}
\end{array}
\right.
$$



### Examples

1. For \( n = 6 \) (even):
   $$
   S_6 = -\frac{6}{2} = -3
   $$

2. For \( n = 5 \) (odd):
   $$
   S_5 = \frac{5+1}{2} = 3
   $$


